example/Fir.CheckN.fst
@@ -1,0 +1,59 @@
+(* This is an example of proving interesting things by mixing induction over lists with proofs about streams. *)
+module Fir.CheckN
+
+open Pipit.Sugar.Vanilla
+module Check = Pipit.Sugar.Check
+
+// open Pipit.System.Base
+open Pipit.System.Ind
+open Pipit.System.Exp
+
+module T = Pipit.Tactics
+
+module R = FStar.Real
+
+let treal = Pipit.Prim.Vanilla.TReal
+
+type fir_contract (mul: R.real) =
+  Check.contract table [treal] treal
+    (Check.exp_of_stream1 (fun i -> abs i <=^ r1))
+    (Check.exp_of_stream2 (fun r i -> abs r <=^ pure mul))
+
+// type fir_contract' (mul: list R.real) =
+//   Check.contract1 table [treal] treal
+//     (fun i -> abs i <=^ r1)
+//     (fun i r -> abs r <=^ pure mul)
+
+let r_abs (r: R.real): R.real =
+  R.(if r >=. zero then r else (zero -. r))
+
+let rec sum_abs (coeffs: list R.real) =
+  match coeffs with
+  | [] -> R.zero
+  | c::cs' -> R.(r_abs c +. sum_abs cs')
+
+#push-options "--print_full_names"
+let rec fir_body (coeffs: list R.real):
+  fir_contract (sum_abs coeffs) =
+  let r = (Check.exp_of_stream1 (fun i -> abs i <=^ r1)) in
+  let g = (Check.exp_of_stream2 (fun r i -> abs r <=^ pure (sum_abs coeffs))) in
+
+  match coeffs with
+  | [] ->
+    let e = Check.exp_of_stream1 (fun _ -> zero) in
+    assume (Check.contract_system_induct_k1' r g e);
+    // assert (Check.contract_system_induct_k1' r g e) by (T.norm_full ());
+    Check.contract_of_exp1 r g e
+  | c :: coeffs' ->
+    let gg = (Check.exp_of_stream2 (fun r i -> abs r <=^ pure R.(r_abs c +. sum_abs coeffs'))) in
+    // assert (g = gg);
+    let e = Check.exp_of_stream1 (fun input ->
+      let fir' = Check.stream_of_contract1 (fir_body coeffs') (fby 0.0R input) in
+      (input *^ pure c) +^ fir') in
+    // assume (Pipit.Exp.Causality.causal r);
+    // assume (Pipit.Exp.Causality.causal gg);
+    // assume (Pipit.Exp.Causality.causal e);
+    // assert (Check.contract_system_induct_k1' r gg e) by (T.norm_full (); T.dump "step");
+    assert (Pipit.System.Ind.base_case (Pipit.System.Exp.system_of_contract r gg e)) by (T.pipit_simplify_products (); T.dump "step");
+    assume (Check.contract_system_induct_k1' r g e);
+    Check.contract_of_exp1 r g e
